Spqr.lean
@@ -64,7 +64,6 @@ import Spqr.Specs.Aeneas.VecIndexRangeFull
 import Spqr.Specs.Authenticator.Authenticator.MACSIZE
 import Spqr.Specs.Authenticator.Serialize.Authenticator.FromPb
 import Spqr.Specs.Authenticator.Serialize.Authenticator.IntoPb
-import Spqr.Specs.CREAM.FromSeed
 import Spqr.Specs.Encoding.Encoder.NextChunk
 import Spqr.Specs.Encoding.Gf.GF16.Add
 import Spqr.Specs.Encoding.Gf.GF16.AddAssign
